â€‹
**Solution:**

Explanation:
- With n is length of the list, will have n! permutation
  n! = n * (n-1) * (n-2) * ... * 1
By example: [1, 2, 3]

We want permutation with length is length of the list, is 3, then we have 3 positions to put value on: _  _  _

- At position 1, permutation = _ _ _ ; choices = [1, 2, 3]
  - If select 1, -> permutation = 1 _ _ ; choices = [2, 3]
    - If select 2 -> permutation = 1 2 _ ; choices = [3]
        - If select 3 -> permutation = 1 2 3 ; choices = [] -> no more choice
            > append permutation [1, 2, 3] to result
    - If select 3 -> permutation = 1 3 _ ; choices = [2]
        - If select 2 -> permutation = 1 3 2 ; choices = [] -> no more choice
            > append permutation [1, 3, 2] to result
  - If select 2, the choices will reduce to [1, 3]
    - If select 1 -> permutation = 2 1 _ ; choices = [3]
        - If select 3 -> permutation = 2 1 3 ; choices = [] -> no more choice
            > append permutation [2, 1, 3] to result
    - If select 3 -> permutation = 2 3 _ ; choices = [1]
        - If select 1 -> permutation = 2 3 1 ; choices = [] -> no more choice
            > append permutation [2, 3, 1] to result
  - If select 3, the choices will reduce to [1, 2]
    - If select 1 -> permutation = 3 1 _ ; choices = [2]
        - If select 2 -> permutation = 3 1 2 ; choices = [] -> no more choice
            > append permutation [3, 1, 2] to result
    - If select 2 -> permutation = 3 2 _ ; choices = [1]
        - If select 1 -> permutation = 3 2 1 ; choices = [] -> no more choice
            > append permutation [3, 2, 1] to result


> If still have choice, get next value and put to permutation, then pop them out of the choices
>
> If no more choice, append permutation to results.
